crates/correctness/lean/MxxCorrectness/Generated/ToyExample/Ir.lean
@@ -11,7 +11,7 @@ def ToyExample_protocolSourceHash : String := "e7b179bba826b3bb584fda61083591285
 
 def ToyExample_workflowHash : String := "1cffc358ce796800fad2b9513f767c5df8e2eaf8e62bca1329a8b0012874b0df"
 
-def ToyExample_toolkitHash : String := "3974c07be50323fae267eaffdbfa4b513fe1070a6c706bd74741686f92ef2d6a"
+def ToyExample_toolkitHash : String := "568403504194710bf4e0845a563878da03ca59213e54bafc2a7f5209b85580f2"
 
 def ToyExample_stage_encrypt : Mxx.Ir.Prog :=
   { root :=
